src/Init/Data/String/Defs.lean
@@ -422,7 +422,7 @@ instance : Inhabited Slice where
 /--
 Returns a slice that contains the entire string.
 -/
-@[inline, expose] -- expose for the defeq `s.toSlice.str = s`.
+@[inline, expose, implicit_reducible] -- expose for the defeq `s.toSlice.str = s`.
 def toSlice (s : String) : Slice where
   str := s
   startInclusive := s.startPos
