src/Std/Data/Iterators/Lemmas/Equivalence/Basic.lean
@@ -96,6 +96,7 @@ coinductive_fixpoint monotonicity by
 
 end Definition
 
+set_option backward.isDefEq.respectTransparency.types false in
 @[simp]
 theorem Equivalence.prun_liftInner_step [Iterator α m β] [Monad m] [Monad n]
     [MonadLiftT m n] [LawfulMonad m] [LawfulMonad n] [LawfulMonadLiftT m n]
@@ -109,6 +110,7 @@ theorem Equivalence.property_step [Iterator α m β] [Monad m] [LawfulMonad m]
     {it : IterM (α := α) m β} : (IterM.stepAsHetT it).Property = it.IsPlausibleStep :=
   rfl
 
+set_option backward.isDefEq.respectTransparency.types false in
 @[simp]
 theorem Equivalence.prun_step [Iterator α m β] [Monad m] [LawfulMonad m]
     {it : IterM (α := α) m β} {f : (step : _) → _ → m γ} :
@@ -240,6 +242,7 @@ theorem Iter.Equiv.trans {α₁ α₂ α₃ β : Type w}
     (hbc : Iter.Equiv itb itc) : Iter.Equiv ita itc :=
   BundledIterM.Equiv.trans hab hbc
 
+set_option backward.isDefEq.respectTransparency.types false in
 theorem IterM.Equiv.of_morphism {α₁ α₂} {m : Type w → Type w'} [Monad m] [LawfulMonad m]
     {β : Type w} [Iterator α₁ m β] [Iterator α₂ m β]
     (ita : IterM (α := α₁) m β)
